Use of Variable and Hypothesis at the top-level to share all the constraints on well-formedness.

transformations/Moore2Mealy/theorems/Elements.v
@@ -6,24 +6,30 @@ Require Moore2Mealy.MealyWF.
 
 Import OptionUtils.
 
+Section Foo.
+
+Variable (m:Moore.M).
+
+Hypothesis WF_U : MooreWF.unique_ids m.
+Hypothesis WF_T : Moore.WF_target m.
+
 Definition convert (s:Moore.State_t) : Mealy.State_t :=
   {| Mealy.State_id := s.(Moore.State_id) |}.
 
 Lemma convert_injective : 
-  forall m s1 s2,
-    MooreWF.unique_ids m ->
+  forall s1 s2,
     List.In (Moore.StateElement s1) m.(Model.modelElements) ->
     List.In (Moore.StateElement s2) m.(Model.modelElements) ->
     convert s1 = convert s2 ->
     s1 = s2.
 Proof.
-  intros m s1 s2 WF H1 H2 H3.
-  apply WF ; auto.
+  intros s1 s2 H1 H2 H3.
+  apply WF_U ; auto.
   destruct s1, s2 ; unfold convert in H3 ; congruence.
 Qed.
 
 
-Definition convert_transition  (m: Moore.M)  (t : Moore.Transition_t)   :option Mealy.Transition_t :=
+Definition convert_transition  (t : Moore.Transition_t)   :option Mealy.Transition_t :=
   match Moore.getTransition_target m t with
   | None => None
   | Some s => Some (Mealy.Build_Transition_t t.(Moore.Transition_id) t.(Moore.Transition_input) s.(Moore.State_output))
@@ -31,9 +37,9 @@ Definition convert_transition  (m: Moore.M)  (t : Moore.Transition_t)   :option 
 
 
 Lemma convert_transition_injective : 
-  forall m t1 t2 a, 
-    convert_transition m t1 = Some a -> (* would be false with None *)
-    convert_transition m t2 = Some a ->
+  forall t1 t2 a, 
+    convert_transition t1 = Some a -> (* would be false with None *)
+    convert_transition t2 = Some a ->
     t1 = t2.
 Proof.
   unfold convert_transition ; intros.
@@ -44,13 +50,12 @@ Proof.
 Qed.
 
 
-Lemma convert_transition_ok : forall (m:Moore.M) t,
-    Moore.WF_target m ->
+Lemma convert_transition_ok : forall t,
     List.In (Moore.TransitionElement t) m.(Model.modelElements) -> 
-    SUCCESS (convert_transition m t).
+    SUCCESS (convert_transition t).
 Proof.
-  intros m t H0 H.
-  apply H0 in H.
+  intros t H.
+  apply WF_T in H.
   destruct H as [s H].
   unfold convert_transition.
   exists (Mealy.Build_Transition_t t.(Moore.Transition_id) t.(Moore.Transition_input) s.(Moore.State_output)).
@@ -66,24 +71,25 @@ Notation transform_element_fw :=
   (Tactics.transform_element_fw  (tc := Moore2Mealy.Moore2MealyTransformationConfiguration)).
 
 Lemma state_element_fw : 
-  forall (s:Moore.State_t) (m:Moore.M),
+  forall (s:Moore.State_t),
     List.In (Moore.StateElement s) (Model.modelElements m) ->
     List.In (Mealy.StateElement (convert s))  (Semantics.execute  Moore2Mealy.Moore2Mealy m).(Model.modelElements).
 Proof.
-  intros s m IN.
+  intros s IN.
   eapply transform_element_fw ; eauto. 
   compute ; auto.
 Qed.
 
 Lemma state_element_bw :
-  forall (s:Mealy.State_t) (m:Moore.M),
+  forall (s:Mealy.State_t),
     List.In (Mealy.StateElement s) (Model.modelElements (Semantics.execute  Moore2Mealy.Moore2Mealy m)) ->
     exists s0,
       List.In (Moore.StateElement s0) (Model.modelElements m) /\ s = convert s0.
 Proof.
-  intros s m H.
+  intros s H.
   core.Tactics.exploit_element_in_result H.
   exists t0.
   split ; auto.
 Qed.
 
+End Foo.
