transformations/Moore2MealyALT/theorems/SemanticPreservation.v
@@ -10,27 +10,30 @@ Require Moore2MealyALT.theorems.StepCommut.
 
 Import String OptionUtils.
 
+Section Foo.
 
-Lemma star_step_commut_fw m :
-  Moore.WF_source m->
-  Moore.WF_target m ->
-  MooreWF.determinist m ->
-  MooreWF.unique_ids m ->
-  
-  forall i s  r,
+Variable (m:Moore.M).
+
+Hypothesis WF_S : Moore.WF_source m.
+Hypothesis WF_T : Moore.WF_target m.
+Hypothesis WF_D : MooreWF.determinist m.
+Hypothesis WF_U : MooreWF.unique_ids m.
+
+
+Lemma star_step_commut_fw :
+  forall i s r,
     MooreSemantics.executeFromState m s i = Some r ->
     MealySemantics.executeFromState
       (Semantics.execute Moore2Mealy.Moore2Mealy m)
       (Elements.convert s) i = Some r.
 Proof.
-  intros WF1 WF2 WF3 WF4.
   induction i ; simpl ; intros s r STEP ; [ congruence | ].
   rename s into s1.
   PropUtils.destruct_match STEP ; [ | discriminate ].
   rename s into s2.
   PropUtils.destruct_match STEP ; [ | discriminate ].
   PropUtils.inj STEP.
-  apply StepCommut.search_commut_fw in Heqo ; auto.
+  apply StepCommut.search_commut_fw in Heqo ; auto. 
   destruct Heqo as (s1' & s2' & ? & ? & t' & ? & ?).
   rewrite <- H.
   rewrite H1.
@@ -42,17 +45,8 @@ Proof.
   assumption.
 Qed.
 
-              
 
-
-
-
-Lemma star_step_commut_bw m :
-  Moore.WF_source m->
-  Moore.WF_target m ->
-  MooreWF.determinist m ->
-  MooreWF.unique_ids m ->
-  
+Lemma star_step_commut_bw :
   forall i s' r,
     MealySemantics.executeFromState
       (Semantics.execute Moore2Mealy.Moore2Mealy m)
@@ -61,7 +55,6 @@ Lemma star_step_commut_bw m :
     exists s, 
       s'= Elements.convert s /\ List.In (Moore.StateElement s) m.(Model.modelElements) /\ MooreSemantics.executeFromState m s i = Some r.
 Proof.
-  intros WF1 WF2 WF3 WF4.
   induction i ; intros s r STEP.
   { 
     simpl in STEP.
@@ -76,52 +69,50 @@ Proof.
     { apply MealySemantics.execute_in in STEP ; auto. discriminate. }
     
     simpl in STEP. simpl.
-  PropUtils.destruct_match STEP ; [ | discriminate ].
-  destruct p.
-  rename s into s2'.
-  PropUtils.destruct_match STEP ; [ | discriminate ].
-  PropUtils.inj STEP.
-  apply StepCommut.search_commut_bw in Heqo ; auto.
-  destruct Heqo as (s1 & ? & s2 & ? & ? & ?).
-  apply Elements.state_element_bw in H.
-  destruct H as (s1_alt & ? & ?).
-
-  assert (s1_alt = s1).
-  { eapply Elements.convert_injective ; eauto.
-    { eapply MooreSemantics.search_in_left ; eauto. }
-    congruence.
-  }
-  subst s1_alt.
-
-  exists s1.
-  split ; [ assumption | ].
-  rewrite H2. 
-  split ; [ assumption | ].
-  specialize (IHi s2' l Heqo0).
-  destruct IHi.
-  { destruct H5 ; subst. simpl.
-    congruence.
-  }
-  destruct H5 as (s2_alt & ? & ? & ?).
-  assert (s2_alt = s2).
-  {
-    eapply Elements.convert_injective ; eauto.
-    eapply MooreSemantics.search_in_right ; eauto.
-    congruence.
-  }
-  subst s2_alt.
-  rewrite H7.
-  f_equal.
-  f_equal.
-  auto.
+    PropUtils.destruct_match STEP ; [ | discriminate ].
+    destruct p.
+    rename s into s2'.
+    PropUtils.destruct_match STEP ; [ | discriminate ].
+    PropUtils.inj STEP.
+    apply StepCommut.search_commut_bw in Heqo ; auto.
+    destruct Heqo as (s1 & ? & s2 & ? & ? & ?).
+    apply Elements.state_element_bw in H.
+    destruct H as (s1_alt & ? & ?).
+    
+    assert (s1_alt = s1).
+    { 
+      eapply Elements.convert_injective ; eauto.
+      { eapply MooreSemantics.search_in_left ; eauto. }
+      { congruence. }
+    }
+    subst s1_alt.
+    
+    exists s1.
+    split ; [ assumption | ].
+    rewrite H2. 
+    split ; [ assumption | ].
+    specialize (IHi s2' l Heqo0).
+    destruct IHi.
+    { 
+      destruct H5 ; subst. simpl.
+      congruence.
+    }
+    destruct H5 as (s2_alt & ? & ? & ?).
+    assert (s2_alt = s2).
+    {
+      eapply Elements.convert_injective ; eauto.
+      eapply MooreSemantics.search_in_right ; eauto.
+      congruence.
+    }
+    subst s2_alt.
+    rewrite H7.
+    f_equal.
+    f_equal.
+    auto.
   }
 Qed.
 
-Lemma SemanticsPreservation m :
-  Moore.WF_source m->
-  Moore.WF_target m ->
-  MooreWF.determinist m ->
-  MooreWF.unique_ids m ->
+Lemma SemanticsPreservation :
   forall i,
     MealySemantics.execute (Semantics.execute Moore2Mealy.Moore2Mealy m) i = MooreSemantics.execute m i.
 Proof. 
@@ -129,7 +120,7 @@ Proof.
   unfold MealySemantics.execute.
   unfold MooreSemantics.execute.
   
-  intros WF1 WF2 WF3 WF4 i .
+  intro i .
   destruct (MooreSemantics.initialState m) eqn:INIT.
   2:{ 
     apply InitStable.initial_state_preserved_fw3 in INIT.
@@ -139,32 +130,36 @@ Proof.
 
   {
     cut (List.In (Moore.StateElement s) m.(Model.modelElements)).
-    intro IN.
-    apply InitStable.initial_state_preserved_fw2 in INIT ; [ | assumption ].
-    rewrite INIT.
-   
-    clear INIT.
-    match goal with [ |- ?A = ?B] => destruct B eqn:? end. 
-
-    + apply star_step_commut_fw in Heqo ; auto.
-    + destruct i.
-      simpl in *.
-      auto.
-      match goal with [ |- ?A = None ] => destruct A eqn:? end ; [ exfalso | reflexivity ].   
-      apply star_step_commut_bw in Heqo0 ; auto.
-      destruct Heqo0.
-      destruct H ; discriminate. 
-      destruct H as (? & ? & ? & ?).
-      eapply Elements.convert_injective in H ; eauto.
-      subst x.
-      congruence.
-
-    + (* inversion *)
+    {
+      intro IN.
+      apply InitStable.initial_state_preserved_fw2 in INIT. 
+      rewrite INIT.
+      
+      clear INIT.
+      match goal with [ |- ?A = ?B] => destruct B eqn:? end. 
+      
+      + apply star_step_commut_fw in Heqo ; auto.
+      + destruct i.
+        simpl in *.
+        auto.
+        match goal with [ |- ?A = None ] => destruct A eqn:? end ; [ exfalso | reflexivity ].   
+        apply star_step_commut_bw in Heqo0 ; auto.
+        destruct Heqo0.
+        destruct H ; discriminate. 
+        destruct H as (? & ? & ? & ?).
+        eapply Elements.convert_injective in H ; eauto.
+        subst x.
+        congruence.
+    }
+    {
+      (* inversion *)
       unfold MooreSemantics.initialState in INIT.
       apply OptionListUtils.find_lift_some in INIT.
       destruct INIT as (?&?&?&?).
       unfold Moore.get_E_data in H ; simpl in H. destruct x ; [ PropUtils.inj H | discriminate H].
       assumption.
+    }
   }
 Qed.
 
+End Foo.
