transformations/Moore2MealyALT/theorems/StepCommut.v
@@ -10,22 +10,25 @@ Require Moore2MealyALT.theorems.GettersCommut.
 
 Import String OptionUtils.
 
+Section Foo.
+
+Variable (m:Moore.M).
+
+Hypothesis WF_S : Moore.WF_source m.
+Hypothesis WF_T : Moore.WF_target m.
+Hypothesis WF_D : MooreWF.determinist m.
 
 (** [State_outTransitions] *)
 
 
-Lemma in_outTransitions_commut_fw m t s t' :
-  Moore.WF_source m ->
-  Moore.WF_target m ->
-  MooreWF.determinist m ->
-
-    List.In t (MooreSemantics.State_outTransitions m s) ->
-    Elements.convert_transition m t = Some t' ->
-    List.In t' (MealySemantics.State_outTransitions
-       (Semantics.execute Moore2Mealy.Moore2Mealy m)
-       (Elements.convert s)).
+Lemma in_outTransitions_commut_fw t s t' :
+  List.In t (MooreSemantics.State_outTransitions m s) ->
+  Elements.convert_transition m t = Some t' ->
+  List.In t' (MealySemantics.State_outTransitions
+                (Semantics.execute Moore2Mealy.Moore2Mealy m)
+                (Elements.convert s)).
 Proof.
-  intros WF1 WF2 WF3. intros.
+  intros.
   destruct (MooreSemantics.State_out_transitions_inv  _ _ _ H).
   apply Elements.transition_element_fw in H1 ; auto.
   destruct H1 as (?&?&?).
@@ -40,18 +43,14 @@ Proof.
 Qed.
 
 
-Lemma in_outTransitions_commut_bw m t s' t' :
-  Moore.WF_source m ->
-  Moore.WF_target m ->
-  MooreWF.determinist m ->
-
-    List.In t' 
-      (MealySemantics.State_outTransitions (Semantics.execute Moore2Mealy.Moore2Mealy m) s') ->
-    Elements.convert_transition m t = Some t' ->
-    exists s, Elements.convert s = s' /\
-    List.In t (MooreSemantics.State_outTransitions m s).
+Lemma in_outTransitions_commut_bw t s' t' :
+  List.In t' 
+    (MealySemantics.State_outTransitions (Semantics.execute Moore2Mealy.Moore2Mealy m) s') ->
+  Elements.convert_transition m t = Some t' ->
+  exists s, Elements.convert s = s'
+            /\ List.In t (MooreSemantics.State_outTransitions m s).
 Proof.
-  intros WF1 WF2 WF3. intros.
+  intros.
   destruct (MealySemantics.State_out_transitions_inv  _ _ _ H).
   apply Elements.transition_element_bw in H1 ; auto.
   destruct H1 as (?&?&?).
@@ -76,17 +75,14 @@ Proof.
     reflexivity.
 Qed.
 
-Lemma in_outTransitions_commut_bw_2 m s' t' :
-  Moore.WF_source m ->
-  Moore.WF_target m ->
-  MooreWF.determinist m ->
-
-    List.In t' 
-      (MealySemantics.State_outTransitions (Semantics.execute Moore2Mealy.Moore2Mealy m) s') ->
-    exists t,  Elements.convert_transition m t = Some t' /\
-    exists s, Elements.convert s = s' /\
-                 
-    List.In t (MooreSemantics.State_outTransitions m s).
+Lemma in_outTransitions_commut_bw_2 s' t' :
+  List.In t' 
+    (MealySemantics.State_outTransitions (Semantics.execute Moore2Mealy.Moore2Mealy m) s') ->
+  exists t,  
+    Elements.convert_transition m t = Some t'
+    /\ exists s,
+      Elements.convert s = s' 
+      /\ List.In t (MooreSemantics.State_outTransitions m s).
 Proof.
   intros.
   cut (exists t : Moore.Transition_t,
@@ -97,20 +93,20 @@ Proof.
     eapply in_outTransitions_commut_bw ; eauto.
   }    
   {
-    destruct (MealySemantics.State_out_transitions_inv  _ _ _ H2).
+    destruct (MealySemantics.State_out_transitions_inv  _ _ _ H).
     unfold Elements.convert_transition.
     cut (Mealy.WF_target (Semantics.execute Moore2Mealy.Moore2Mealy m)) ; auto with wf.
     intro WF.
-    destruct  (WF _ H3).
-    eapply GettersCommut.getTransition_target_commut_bw in H5 ; eauto.
-    destruct H5 as (t & ?& ?& ? & ?).
+    destruct  (WF _ H0).
+    eapply GettersCommut.getTransition_target_commut_bw in H2 ; eauto.
+    destruct H2 as (t & ?& ?& ? & ?).
     exists t.
-    rewrite H7.
+    rewrite H4.
     subst.
     f_equal.
-    unfold Elements.convert_transition in H5.
-    rewrite H7 in H5.
-    PropUtils.inj H5.
+    unfold Elements.convert_transition in H2.
+    rewrite H4 in H2.
+    PropUtils.inj H2.
     reflexivity.
   }
 Qed.
@@ -119,20 +115,17 @@ Qed.
 (** [State_acceptTransition] *)
 
 Lemma State_acceptTransition_commut_fw :
-  forall s m i t,
-    Moore.WF_source m ->
-    Moore.WF_target m ->
-    MooreWF.determinist m ->
+  forall s i t,
     MooreSemantics.State_acceptTransition m s i = Some t ->
     MealySemantics.State_acceptTransition (Semantics.execute Moore2Mealy.Moore2Mealy m) (Elements.convert s) i = Elements.convert_transition m t.
 Proof.
-  intros s m i t WF_1 WF_2 WF_3 A.
+  intros s i t A.
 
   destruct (MooreSemantics.State_acceptTransition_inv _ _ _ _ A).
   
   destruct (MooreSemantics.State_out_transitions_inv  _ _ _ H). 
   unfold Elements.convert_transition.
-  destruct (WF_2 _ H1) as (s' & H4).
+  destruct (WF_T _ H1) as (s' & H4).
   rewrite H4.
   apply MealyWF.State_acceptTransition_some ; auto with wf.
 
@@ -143,31 +136,28 @@ Proof.
 Qed.
 
 Lemma State_acceptTransition_commut_bw :
-  forall s' m i t',
-    Moore.WF_source m ->
-    Moore.WF_target m ->
-    MooreWF.determinist m ->
+  forall s' i t',
     MealySemantics.State_acceptTransition (Semantics.execute Moore2Mealy.Moore2Mealy m) s' i = Some t' ->
-
-    exists s, Elements.convert s = s' /\ 
-                exists t,
-                  Elements.convert_transition m t = Some t' /\
-                    MooreSemantics.State_acceptTransition m s i = Some t 
-    .
+    
+    exists s, 
+      Elements.convert s = s' 
+      /\ exists t,
+        Elements.convert_transition m t = Some t' 
+        /\ MooreSemantics.State_acceptTransition m s i = Some t.
 Proof.
   intros.
 
-  destruct (MealySemantics.State_acceptTransition_inv _ _ _ _ H2).
+  destruct (MealySemantics.State_acceptTransition_inv _ _ _ _ H).
 
-  eapply in_outTransitions_commut_bw_2 in H3 ; eauto.
-  destruct H3 as (t&?& s & ? & ?).
+  eapply in_outTransitions_commut_bw_2 in H0 ; eauto.
+  destruct H0 as (t&?& s & ? & ?).
   exists s ; split ; auto.
   exists t ; split ; auto.
   unfold MooreSemantics.State_acceptTransition.
   apply ListUtils.in_find ; eauto.
   { apply MooreWF.truc. assumption. }
   { apply String.eqb_eq.
-    destruct (Elements.convert_transition_inv _ _ _ H3) as (?& _ &?).
+    destruct (Elements.convert_transition_inv _ _ _ H0) as (?& _ &?).
     subst.
     reflexivity.
   }
@@ -175,19 +165,16 @@ Qed.
 
 (** [ search] *)
 
-Lemma search_commut_fw m :
-  Moore.WF_source m ->
-  Moore.WF_target m ->
-  MooreWF.determinist m ->
+Lemma search_commut_fw :
   forall s1 i s2,
     MooreSemantics.search m s1 i = Some s2 ->
     exists s1' s2',
-      s1'= Elements.convert s1 /\
-        s2'= Elements.convert s2 /\ 
-        exists t',
-          MealySemantics.search (Semantics.execute Moore2Mealy.Moore2Mealy m) s1' i = Some (t',s2') /\ Mealy.Transition_output t' = Moore.State_output s2.
+      s1'= Elements.convert s1 
+      /\ s2'= Elements.convert s2 
+      /\ exists t',
+        MealySemantics.search (Semantics.execute Moore2Mealy.Moore2Mealy m) s1' i = Some (t',s2') 
+        /\ Mealy.Transition_output t' = Moore.State_output s2.
 Proof.    
-  intros WF1 WF2 WF3.
   intros.
   
   destruct (MooreSemantics.search_inv _ _ _ _ H) as (?&?&?).
@@ -198,7 +185,7 @@ Proof.
   apply State_acceptTransition_commut_fw in H0 ; auto.
   unfold Elements.convert in H0.
   rewrite H0.
-  destruct (GettersCommut.getTransition_target_commut_fw _ _ WF2 _ H1).
+  destruct (GettersCommut.getTransition_target_commut_fw _ _ _ H1).
 
   rewrite H2.
 
@@ -207,25 +194,23 @@ Proof.
   eauto.
 Qed.
 
-Lemma search_commut_bw m :
-  Moore.WF_source m ->
-  Moore.WF_target m ->
-  MooreWF.determinist m ->
+Lemma search_commut_bw :
   forall s1' i s2' t',
  MealySemantics.search (Semantics.execute Moore2Mealy.Moore2Mealy m) s1' i = Some (t',s2') ->
     exists s1,
-      s1'= Elements.convert s1 /\
-        exists s2, 
-          s2'= Elements.convert s2 /\ 
-            MooreSemantics.search m s1 i = Some s2 /\ Mealy.Transition_output t' = Moore.State_output s2.        
+      s1'= Elements.convert s1 
+      /\ exists s2, 
+        s2'= Elements.convert s2 
+        /\ MooreSemantics.search m s1 i = Some s2 
+        /\ Mealy.Transition_output t' = Moore.State_output s2.        
 Proof.    
-  intros WF1 WF2 WF3 ; intros.
+  intros.
   
   destruct (MealySemantics.search_inv _ _ _ _ _ H).
 
   unfold MooreSemantics.search.
   
-  destruct (State_acceptTransition_commut_bw _ _ _ _ WF1 WF2 WF3 H0) as (s1 & ? & t & ? & ?).
+  destruct (State_acceptTransition_commut_bw  _ _ _ H0) as (s1 & ? & t & ? & ?).
 
   exists s1. split ; auto.
   rewrite H4.
@@ -234,7 +219,7 @@ Proof.
   
   destruct (MealySemantics.State_out_transitions_inv _ _ _ H5).
 
-  destruct (GettersCommut.getTransition_target_commut_bw _ WF2 _ _ H7 H1) as (?&?&s2&?&?).
+  destruct (GettersCommut.getTransition_target_commut_bw _ WF_T _ _ H7 H1) as (?&?&s2&?&?).
   replace x with t in *.
   2:{ eapply Elements.convert_transition_injective ; eauto. }
   clear H8. (* duplicate *)
@@ -245,3 +230,6 @@ Proof.
   PropUtils.inj H8.
   eauto.
 Qed.
+
+
+End Foo.
